Modification of global state

GlobalState.fst
@@ -4,7 +4,7 @@ open FStar.String
 
 (* 
     New type string_66 that only allows strings with 66 characters
-    effectively simulating hexadecimal number of length 64 (+ '0x') == 256 bit number
+    effectively simulating hexadecimal number of length 64 (+ '0x') == 256 bit number == 32 bytes
 *)
 type string_66 = s:string {length s = 66}   // another way to represent 32byte values
 
@@ -12,9 +12,56 @@ let default_string_66 : string_66 =
     let def_str = "0x0000000000000000000000000000000000000000000000000000000000000000" in
     let _ = assume(String.length def_str = 66) in 
     def_str
-// Add relevant event for reforge
-// event Reforged(address indexed account, uint256 amount, string indexed transaction);
-// event Transfer(address indexed from, address indexed to, uint256 value);
+
+(*
+    Default address for roles
+*)
+let multiSigTreasury : address = to_address 0xaB23968d766D445BC9b370512d3085c345AcB235
+
+(*
+    Define creator address for msg.sender - address that has initialized the contract
+    (Info from https://etherscan.io/address/0x3ac694ad2a9a616b6af4fc7e13ab08793eecaac7#code)
+*)
+let original_msg_sender : address = to_address 0x26c09DCd572Ec41dd55Ee099dB9a321E3B34b351
+
+
+(*
+Calculated keccak256("PAUSER_ROLE") from https://emn178.github.io/online-tools/keccak_256.html 
+*)
+let pauser_keccak : string_66 = 
+    let def_str = "0x65d7a28e3265b37a6474929f336521b332c1681b933f6cb9f3376673440d862a" in 
+    let _ = assume(String.length def_str = 66) in 
+    def_str
+
+(*
+Calculated keccak256("MINTER_ROLE") from https://emn178.github.io/online-tools/keccak_256.html
+*)
+let minter_keccak : string_66 = 
+    let def_str = "0x9f2df0fed2c77648de5860a4cc508cd0818c85b8b8a1ab4ceeef8d981c8956a6" in 
+    let _ = assume(String.length def_str = 66) in 
+    def_str
+
+(*
+Calculated keccak256("UPGRADER_ROLE") from https://emn178.github.io/online-tools/keccak_256.html 
+*)
+let upgrader_keccak : string_66 = 
+    let def_str = "0x189ab7a9244df0848122154315af71fe140f3db0fe014031783b0946b8c9d2e3" in 
+    let _ = assume(String.length def_str = 66) in 
+    def_str
+
+(*
+Calculated keccak256("BRIDGE_OWNER_ROLE") from https://emn178.github.io/online-tools/keccak_256.html 
+*)
+let bridger_owner_keccak : string_66 = 
+    let def_str = "0xca93eeebffcc91aeddd69986d2392810138feb62c9e4efc6996600ed00e90b6d" in 
+    let _ = assume(String.length def_str = 66) in 
+    def_str
+
+(* 
+    Relevant events:
+        - event Reforged(address indexed account, uint256 amount, string indexed transaction);
+        - event Transfer(address indexed from, address indexed to, uint256 value);
+*)
 type event = 
     | Reforged : address -> uint -> string_66 -> event
     | Transfer : address -> address -> uint -> event
@@ -49,49 +96,91 @@ noeq type _RoleData = {
 
 noeq type global_state = {
     (* list of events *)
-    events_         : list event;
+    events_             : list event;
 
     (* mapping transaction string (transaction hash) to bool
        bool is by default set to `false` *)
-    _transactions   : string_66 -> bool;
+    _transactions       : string_66 -> bool;
 
     (* type that contains all role hashes (keccak256 hashes) *)
-    roles           : role;
+    roles               : role;
 
     (* mapping role hashes (keccak256 hashes) into _RoleData struct *)
-    _roles          : string_66 -> _RoleData;  
+    _roles              : string_66 -> _RoleData;  
 
     (* uint that presents the total number of tokens in the existence
        essentially it presents all tokens that were ever minted *)
-    _totalSupply    : uint;
+    _totalSupply        : uint;
 
     (* mapping address to uint (representing the balance of tokens for specific account) *)
-    _balances       : address -> uint;
+    _balances           : address -> uint;
 
     (* address that receives transaction fees in native currency *)
-    _bridgeOwner    : address;
+    _bridgeOwner        : address;
 
     (* boolean variable, indicates if contract is paused *)
-    _paused         : bool; 
+    _paused             : bool; 
 
+    (* boolean variable, indicates if bridge is paused *)
+    _bridgePaused       : bool;
+
+    (* uint that presents the bridge transacion fee in native currency *)
+    _minimumBridgeFee   : uint;
+
+    (* mapping chain_id (uint) to the address of the specific token e.g., eEUR *)
+    (* Example: maps Ethereum_chain to eEUR token *)
+    _sameTokens         : uint -> address;
+
+    (* uint that presents the minimal required amount for SendToChain *)
+    _minimumSendToChainAmount   : uint;
+
+    (* address of feeTresury *)
+    _feeTreasury        : address;
+
+    (* uint that presetns the bridge transaction fee percentage (10^6 == 1%) *)
+    _bridgeFee          : uint;
 }
 
 let default_state : global_state = {
     events_         = [];
     _transactions   = ( fun x -> false );
     roles           = {
-                        _PAUSER_ROLE        = default_string_66;
-                        _MINTER_ROLE        = default_string_66;
-                        _UPGRADER_ROLE      = default_string_66;
-                        _BRIDGE_OWNER_ROLE  = default_string_66;
-                        _ADMIN_eEUR         = default_string_66;
+                        _PAUSER_ROLE        = pauser_keccak;        (* symulating keccak256("PAUSER_ROLE") *)
+                        _MINTER_ROLE        = minter_keccak;        (* symulating keccak256("MINTER_ROLE") *)
+                        _UPGRADER_ROLE      = upgrader_keccak;      (* symulating keccak256("UPGRADER_ROLE") *)
+                        _BRIDGE_OWNER_ROLE  = bridger_owner_keccak; (* symulating keccak256("BRIDGE_OWNER_ROLE") *)
+                        _ADMIN_eEUR         = default_string_66;    (* default 0x00 *)
     };
-    _roles          = ( fun role -> { 
+    (*_roles          = ( fun role -> { 
                                         members = ( fun addr -> false ); 
                                         adminRole = default_string_66 
-                                    });    
+                                    }); *)
+    (* Add default account for reoles *)
+    _roles          = ( fun role -> { 
+                                        members = ( fun addr ->
+                                                        if      (* role == _PAUSER_ROLE and addr = multiSigTreasury *)
+                                                                (role = pauser_keccak  && addr = multiSigTreasury)
+                                                                (* role == _MINTER_ROLE and addr = multiSigTreasury *)
+                                                            ||  (role = minter_keccak  && addr = multiSigTreasury)
+                                                                (* role == _UPGRADER_ROLE and addr = multiSigTreasury *)
+                                                            ||  (role = upgrader_keccak && addr = multiSigTreasury)
+                                                                (* role == _BRIDGE_OWNER_ROLE and addr = multiSigTreasury *)
+                                                            ||  (role = bridger_owner_keccak && addr = multiSigTreasury)
+                                                                (* role == _ADMIN_eEUR and addr = creator of the contract *)
+                                                            ||  (role = default_string_66 && addr = original_msg_sender) 
+                                                        then true
+                                                        else false ); 
+                                        adminRole = default_string_66 (* _ADMIN_eEUR  *)
+                                    });
     _totalSupply    = Solidity.to_uint 0;
     _balances       = ( fun x -> Solidity.to_uint 0   );
     _bridgeOwner    = default_address;
     _paused         = false;
+    _bridgePaused   = false;
+    _minimumBridgeFee   = Solidity.to_uint 0;           
+    _sameTokens     = ( fun x -> default_address );     // TODO
+    // Ether_chain = 137 | eEUR (0x735fa792e731a2e8F83F32eb539841b7B72e6d8f) - https://etherscan.io/tx/0xc81b5f69aeda6eaa159f244d3aa5ae56a905c336b455f6dd37675937ef4f7c26 
+    _minimumSendToChainAmount   = Solidity.to_uint 10000000000000000000000;   (* default value is 10^22 *)
+    _feeTreasury    = multiSigTreasury;
+    _bridgeFee      = Solidity.to_uint 300000; (* 300000 == 0.3% *)
 }
